CBOR verified C test: build a map

src/cbor/pulse/det/vertest/c/CBORTest.fst
@@ -4,6 +4,17 @@ open CBOR.Pulse.API.Det.C
 module C = C
 open Pulse.Lib.Pervasives
 module A = Pulse.Lib.Array
+module SZ = FStar.SizeT
+module U8 = FStar.UInt8
+module SM = Pulse.Lib.SeqMatch.Util
+module Trade = Pulse.Lib.Trade.Util
+
+inline_for_extraction
+noextract [@@noextract_to "krml"]
+let letter (x: U8.t { 1 <= U8.v x /\ U8.v x <= 26 }) : U8.t =
+  U8.add 96uy x
+
+#push-options "--fuel 8"
 
 ```pulse
 fn main (_: unit)
@@ -11,8 +22,50 @@ requires emp
 returns res: C.exit_code
 ensures pure (res == C.EXIT_SUCCESS)
 {
-  let dummy_cbor = cbor_det_mk_int64 () cbor_major_type_uint64 18uL;
-  drop_ (cbor_det_match _ dummy_cbor _);
+  let mut foo0 = [| letter 6uy; 3sz |];
+  foo0.(1sz) <- letter 15uy;
+  foo0.(2sz) <- letter 15uy;
+  with foo_v . assert (A.pts_to foo0 foo_v);
+  let foo = cbor_det_mk_string_from_array () cbor_major_type_byte_string foo0 3uL;
+  let i18 = cbor_det_mk_int64' cbor_major_type_uint64 18uL;
+  let foo_i18 = cbor_det_mk_map_entry () foo i18;
+  Trade.trans_concl_l (cbor_det_map_entry_match 1.0R foo_i18 _) _ _ _;
+  Trade.trans_concl_r (cbor_det_map_entry_match 1.0R foo_i18 _) _ _ _;
+  let mut map_entries = [| foo_i18; 3sz |];
+  let mut bar0 = [| letter 2uy; 3sz |];
+  bar0.(1sz) <- letter 1uy;
+  bar0.(2sz) <- letter 18uy;
+  with bar_v . assert (A.pts_to bar0 bar_v);
+  assert (pure (~ (Seq.index foo_v 0 == Seq.index bar_v 0))); // necessary to prove that foo <> bar
+  let bar = cbor_det_mk_string_from_array () cbor_major_type_byte_string bar0 3uL;
+  let i42 = cbor_det_mk_int64' cbor_major_type_neg_int64 42uL;
+  let bar_i42 = cbor_det_mk_map_entry () bar i42;
+  Trade.trans_concl_l (cbor_det_map_entry_match 1.0R bar_i42 _) _ _ _;
+  Trade.trans_concl_r (cbor_det_map_entry_match 1.0R bar_i42 _) _ _ _;
+  map_entries.(1sz) <- bar_i42;
+  let i1729 = cbor_det_mk_int64' cbor_major_type_uint64 1729uL;
+  let mut quux0 = [| letter 17uy; 4sz |];
+  quux0.(1sz) <- letter 21uy;
+  quux0.(2sz) <- letter 21uy;
+  quux0.(3sz) <- letter 24uy;
+  let quux = cbor_det_mk_string_from_array () cbor_major_type_byte_string quux0 4uL;
+  let i1729_quux = cbor_det_mk_map_entry () i1729 quux;
+  Trade.trans_concl_l (cbor_det_map_entry_match 1.0R i1729_quux _) _ _ _;
+  Trade.trans_concl_r (cbor_det_map_entry_match 1.0R i1729_quux _) _ _ _;
+  map_entries.(2sz) <- i1729_quux;
+  SM.seq_list_match_singleton_intro_trade i1729_quux _ (cbor_det_map_entry_match 1.0R);
+  Trade.trans _ (cbor_det_map_entry_match 1.0R i1729_quux _) _;
+  SM.seq_list_match_cons_intro_trade bar_i42 _ _ _ (cbor_det_map_entry_match 1.0R);
+  Trade.trans_concl_r _ (cbor_det_map_entry_match 1.0R bar_i42 _) _ _;
+  Trade.trans_concl_l _ (cbor_det_map_entry_match 1.0R bar_i42 _) _ _;
+  SM.seq_list_match_cons_intro_trade foo_i18 _ _ _ (cbor_det_map_entry_match 1.0R);
+  Trade.trans_concl_r _ (cbor_det_map_entry_match 1.0R foo_i18 _) _ _;
+  Trade.trans_concl_l _ (cbor_det_map_entry_match 1.0R foo_i18 _) _ _;
+  let map0 = cbor_det_mk_map_from_array' map_entries 3uL _;
+  Trade.trans_concl_r (cbor_det_match _ map0 _) _ _ _;
+  let map = cbor_det_reset_perm () map0;
+  Trade.trans (cbor_det_match 1.0R map _) _ _;
+  Trade.elim (cbor_det_match 1.0R map _) _;
   C.EXIT_SUCCESS
 }
 ```
